coq/ZF/Meta/Test/Set/Pair.v
@@ -1,114 +1,178 @@
 Require Import Coq.Lists.List.
 Require Import Coq.Strings.String.
 
-Require Import ZF.Meta.Ctx.
-Require Import ZF.Meta.Env.
 Require Import ZF.Meta.Check.
+Require Import ZF.Meta.Proof.CheckDecl.
+Require Import ZF.Meta.Proof.Decl.
 Require Import ZF.Meta.Syntax.
+Require Import ZF.Meta.Term.CheckDecl.
 Require Import ZF.Meta.Ty.
 
-Require Import ZF.Meta.Decl.Class.Equiv.
-Require Import ZF.Meta.Decl.Class.Incl.
 Require Import ZF.Meta.Decl.Set.Pair.
 
 Import ListNotations.
 
-(* Environment.                                                                 *)
+(* Declaration typing.                                                          *)
 
-Definition env : Env := Env.unions
-  [ Pair.env
-  ; Incl.env
-  ; Equiv.env
-  ].
-
-(* Propositions.                                                                *)
-
-(* Proposition Charac : forall a b, forall x, x :< pair a b <-> x = a \/ x = b. *)
-Definition Charac : Term :=
-  All VarTySet
-    (All VarTySet
-      (All VarTySet
-        (Iff
-          (Elem (Var 0) (IdentT "pair" [Var 2; Var 1]))
-          (Or
-            (Equal (Var 0) (Var 2))
-            (Equal (Var 0) (Var 1)))))).
-
-(* Proposition IsInL : forall a b, a :< pair a b.                               *)
-Definition IsInL : Term :=
-  All VarTySet
-    (All VarTySet
-      (Elem (Var 1) (IdentT "pair" [Var 1; Var 0]))).
-
-(* Proposition IsInR : forall a b, b :< pair a b.                               *)
-Definition IsInR : Term :=
-  All VarTySet
-    (All VarTySet
-      (Elem (Var 0) (IdentT "pair" [Var 1; Var 0]))).
-
-(* Proposition ToClassIncl : forall A a b,                                      *)
-(* A a /\ A b <-> Incl (toClass (pair a b)) A.                                  *)
-Definition ToClassIncl : Term :=
-  All VarTyClass
-    (All VarTySet
-      (All VarTySet
-        (Iff
-          (And
-            (App (Var 2) (Var 1))
-            (App (Var 2) (Var 0)))
-          (IdentT "Incl"
-            [IdentT "toClass" [IdentT "pair" [Var 1; Var 0]]; Var 2])))).
-
-(* Proposition typing.                                                          *)
-
-(* The characterization of membership in a pair is well sorted.                 *)
-Proposition CharacCheck : CheckT env Ctx.empty Charac TyProp.
+(* The declaration body for IsPairOf recognizes the two selected sets.          *)
+Proposition IsPairOf : CheckDeclT (Pair.env) Pair.IsPairOf.
 Proof.
   (* Proof by Hermes + gpt 5.5                                                  *)
-  apply CheckAll, CheckAll, CheckAll, CheckIff.
-  - apply CheckElem.
-    + apply CheckVar. reflexivity.
-    + apply pairCheckIdent; reflexivity.
+  apply CheckLam, CheckAll, CheckIff.
+  - apply CheckElem; apply CheckVar; reflexivity.
   - apply CheckOr; apply CheckEqual; apply CheckVar; reflexivity.
 Qed.
 
-(* The left element belongs to its pair, and it is well sorted.                 *)
-Proposition IsInLCheck : CheckT env Ctx.empty IsInL TyProp.
+(* The existence proof declaration is well sorted.                              *)
+Proposition Exists : CheckDeclP (Pair.env) Pair.Exists.
 Proof.
   (* Proof by Hermes + gpt 5.5                                                  *)
-  apply CheckAll, CheckAll, CheckElem.
-  - apply CheckVar. reflexivity.
-  - apply pairCheckIdent; reflexivity.
-Qed.
-
-(* The right element belongs to its pair, and it is well sorted.                *)
-Proposition IsInRCheck : CheckT env Ctx.empty IsInR TyProp.
-Proof.
-  (* Proof by Hermes + gpt 5.5                                                  *)
-  apply CheckAll, CheckAll, CheckElem.
-  - apply CheckVar. reflexivity.
-  - apply pairCheckIdent; reflexivity.
-Qed.
-
-(* Containment of both elements and class inclusion are well sorted.            *)
-Proposition ToClassInclCheck : CheckT env Ctx.empty ToClassIncl TyProp.
-Proof.
-  (* Proof by Hermes + gpt 5.5                                                  *)
-  apply CheckAll, CheckAll, CheckAll, CheckIff.
-  - apply CheckAnd.
-    + apply CheckApp.
-      * apply CheckVar. reflexivity.
-      * apply CheckVar. reflexivity.
-    + apply CheckApp.
-      * apply CheckVar. reflexivity.
-      * apply CheckVar. reflexivity.
-  - apply CheckIdentT with [TyClass;TyClass]. 1: reflexivity.
-    apply CheckTsCons.
-    + apply CheckIdentT with [TySet]. 1: reflexivity.
+  assert (CheckT (Pair.env) (ctxP Pair.Exists)
+    (conclP Pair.Exists) TyProp) as H1. {
+    apply CheckEx, CheckApp.
+    - apply CheckIdentT with [TySet;TySet]. 1: reflexivity.
       apply CheckTsCons.
-      * apply pairCheckIdent; reflexivity.
-      * apply CheckTsNil.
+      + apply CheckVar. reflexivity.
+      + apply CheckTsCons.
+        * apply CheckVar. reflexivity.
+        * apply CheckTsNil.
+    - apply CheckVar. reflexivity. }
+  split. 1: assumption. apply CheckHoleP. assumption.
+Qed.
+
+(* The uniqueness proof declaration is well sorted.                             *)
+Proposition Unique : CheckDeclP (Pair.env) Pair.Unique.
+Proof.
+  (* Proof by Hermes + gpt 5.5                                                  *)
+  assert (CheckT (Pair.env) (ctxP Pair.Unique)
+    (conclP Pair.Unique) TyProp) as H1. {
+    apply CheckAll, CheckAll, CheckImp.
+    - apply CheckApp.
+      + apply CheckIdentT with [TySet;TySet]. 1: reflexivity.
+        apply CheckTsCons.
+        * apply CheckVar. reflexivity.
+        * apply CheckTsCons.
+          -- apply CheckVar. reflexivity.
+          -- apply CheckTsNil.
+      + apply CheckVar. reflexivity.
+    - apply CheckImp.
+      + apply CheckApp.
+        * apply CheckIdentT with [TySet;TySet]. 1: reflexivity.
+          apply CheckTsCons.
+          -- apply CheckVar. reflexivity.
+          -- apply CheckTsCons.
+             ++ apply CheckVar. reflexivity.
+             ++ apply CheckTsNil.
+        * apply CheckVar. reflexivity.
+      + apply CheckEqual; apply CheckVar; reflexivity. }
+  split. 1: assumption. apply CheckHoleP. assumption.
+Qed.
+
+(* The declaration body for pair denotes a set backed by proof references.      *)
+Proposition pair : CheckDeclT (Pair.env) Pair.pair.
+Proof.
+  (* Proof by Hermes + gpt 5.5                                                  *)
+  eapply CheckDef. (* TODO: replace 'eapply' with 'apply' *)
+  - apply CheckIdentT with [TySet;TySet]. 1: reflexivity.
+    apply CheckTsCons.
+    + apply CheckVar. reflexivity.
     + apply CheckTsCons.
       * apply CheckVar. reflexivity.
       * apply CheckTsNil.
+  - apply CheckIdentP with [TySet;TySet]. 1: reflexivity.
+    apply CheckTsCons.
+    + apply CheckVar. reflexivity.
+    + apply CheckTsCons.
+      * apply CheckVar. reflexivity.
+      * apply CheckTsNil.
+  - apply CheckIdentP with [TySet;TySet]. 1: reflexivity.
+    apply CheckTsCons.
+    + apply CheckVar. reflexivity.
+    + apply CheckTsCons.
+      * apply CheckVar. reflexivity.
+      * apply CheckTsNil.
+Qed.
+
+(* The characterization proposition is well sorted.                             *)
+Proposition Charac : CheckDeclP (Pair.env) Pair.Charac.
+Proof.
+  (* Proof by Hermes + gpt 5.5                                                  *)
+  assert (CheckT (Pair.env) (ctxP Pair.Charac)
+    (conclP Pair.Charac) TyProp) as H1. {
+    apply CheckAll, CheckAll, CheckAll, CheckIff.
+    - apply CheckElem.
+      + apply CheckVar. reflexivity.
+      + apply CheckIdentT with [TySet;TySet]. 1: reflexivity.
+        apply CheckTsCons.
+        * apply CheckVar. reflexivity.
+        * apply CheckTsCons.
+          -- apply CheckVar. reflexivity.
+          -- apply CheckTsNil.
+    - apply CheckOr; apply CheckEqual; apply CheckVar; reflexivity. }
+  split. 1: assumption. apply CheckHoleP. assumption.
+Qed.
+
+(* The left membership proposition is well sorted.                              *)
+Proposition IsInL : CheckDeclP (Pair.env) Pair.IsInL.
+Proof.
+  (* Proof by Hermes + gpt 5.5                                                  *)
+  assert (CheckT (Pair.env) (ctxP Pair.IsInL)
+    (conclP Pair.IsInL) TyProp) as H1. {
+    apply CheckAll, CheckAll, CheckElem.
+    - apply CheckVar. reflexivity.
+    - apply CheckIdentT with [TySet;TySet]. 1: reflexivity.
+      apply CheckTsCons.
+      + apply CheckVar. reflexivity.
+      + apply CheckTsCons.
+        * apply CheckVar. reflexivity.
+        * apply CheckTsNil. }
+  split. 1: assumption. apply CheckHoleP. assumption.
+Qed.
+
+(* The right membership proposition is well sorted.                             *)
+Proposition IsInR : CheckDeclP (Pair.env) Pair.IsInR.
+Proof.
+  (* Proof by Hermes + gpt 5.5                                                  *)
+  assert (CheckT (Pair.env) (ctxP Pair.IsInR)
+    (conclP Pair.IsInR) TyProp) as H1. {
+    apply CheckAll, CheckAll, CheckElem.
+    - apply CheckVar. reflexivity.
+    - apply CheckIdentT with [TySet;TySet]. 1: reflexivity.
+      apply CheckTsCons.
+      + apply CheckVar. reflexivity.
+      + apply CheckTsCons.
+        * apply CheckVar. reflexivity.
+        * apply CheckTsNil. }
+  split. 1: assumption. apply CheckHoleP. assumption.
+Qed.
+
+(* The class-inclusion proposition is well sorted.                              *)
+Proposition ToClassIncl : CheckDeclP (Pair.env) Pair.ToClassIncl.
+Proof.
+  (* Proof by Hermes + gpt 5.5                                                  *)
+  assert (CheckT (Pair.env) (ctxP Pair.ToClassIncl)
+    (conclP Pair.ToClassIncl) TyProp) as H1. {
+    apply CheckAll, CheckAll, CheckAll, CheckIff.
+    - apply CheckAnd.
+      + apply CheckApp.
+        * apply CheckVar. reflexivity.
+        * apply CheckVar. reflexivity.
+      + apply CheckApp.
+        * apply CheckVar. reflexivity.
+        * apply CheckVar. reflexivity.
+    - apply CheckIdentT with [TyClass;TyClass]. 1: reflexivity.
+      apply CheckTsCons.
+      + apply CheckIdentT with [TySet]. 1: reflexivity.
+        apply CheckTsCons.
+        * apply CheckIdentT with [TySet;TySet]. 1: reflexivity.
+          apply CheckTsCons.
+          -- apply CheckVar. reflexivity.
+          -- apply CheckTsCons.
+             ++ apply CheckVar. reflexivity.
+             ++ apply CheckTsNil.
+        * apply CheckTsNil.
+      + apply CheckTsCons.
+        * apply CheckVar. reflexivity.
+        * apply CheckTsNil. }
+  split. 1: assumption. apply CheckHoleP. assumption.
 Qed.
